haetae-topdown-easycrypt/easycrypt/refinement/keygen/Mode2KeygenCoreEquation.ec
@@ -1,0 +1,330 @@
+require import AllCore IntDiv.
+
+from Jasmin require import JModel_x86.
+
+require import BArray8192 BArray32768
+               Fq Rq
+               KeygenMode2ParentTarget
+               KeygenM23MatrixSpec KeygenM23ArithmeticSpec
+               KeygenM23FinalizeSpec KeygenM23FinalizeSemantics
+               KeygenM23FinalizeArraySemantics
+               KeygenM23FinalizeHAETAEBridge
+               TargetKeygenM23Arithmetic TargetKeygenM23Finalize
+               Mode2KeygenSnapshotAlgebra.
+
+theory Mode2KeygenCoreEquation.
+
+module Parent = KeygenMode2ParentTarget.M.
+
+op centered_s2_active (s2 : BArray8192.t) : bool =
+  forall i,
+    0 <= i < KeygenM23MatrixSpec.mode2_b_words_i =>
+    -1 <= W32.to_sint (BArray8192.get32 s2 i) <= 1.
+
+op canonical_a_active (a : BArray8192.t) : bool =
+  forall i,
+    0 <= i < KeygenM23MatrixSpec.mode2_b_words_i =>
+    W32.to_uint (BArray8192.get32 a i) <
+      KeygenM23FinalizeSemantics.q.
+
+lemma mode2_output_repr_bound16_word
+    (bp : BArray8192.t)
+    (mat : BArray32768.t)
+    (p0 p1 p2 : Rq.poly) i :
+  KeygenM23ArithmeticSpec.mode2_output_repr_bound16
+    bp mat p0 p1 p2 =>
+  0 <= i < KeygenM23MatrixSpec.mode2_b_words_i =>
+  Fq.bw32 (BArray8192.get32 bp i) 16.
+proof.
+move=> hout hi.
+move: hout.
+rewrite /KeygenM23ArithmeticSpec.mode2_output_repr_bound16
+        /KeygenM23ArithmeticSpec.wide_slice_repr_bound
+        /KeygenM23ArithmeticSpec.wide_slice_bound.
+move=> [[_ hb0] [_ hb1]].
+case (i < KeygenM23MatrixSpec.poly_words_i).
++ move=> hi0.
+  have h := hb0 i _.
+  + smt().
+  by move: h; rewrite add0z.
++ move=> hi0.
+  have hj :
+      0 <= i - KeygenM23MatrixSpec.poly_words_i <
+        KeygenM23MatrixSpec.poly_words_i.
+  + move: hi hi0.
+    rewrite /KeygenM23MatrixSpec.mode2_b_words_i
+            /KeygenM23MatrixSpec.mode2_rows_i
+            /KeygenM23MatrixSpec.poly_words_i.
+    smt().
+  have h := hb1 (i - KeygenM23MatrixSpec.poly_words_i) hj.
+  have heq :
+      KeygenM23MatrixSpec.poly_words_i +
+        (i - KeygenM23MatrixSpec.poly_words_i) = i by ring.
+  by move: h; rewrite heq.
+qed.
+
+lemma finalize_reachable_inputs_from_matrix_output
+    (bp s2 a : BArray8192.t)
+    (mat : BArray32768.t)
+    (p0 p1 p2 : Rq.poly) :
+  KeygenM23ArithmeticSpec.mode2_output_repr_bound16
+    bp mat p0 p1 p2 =>
+  centered_s2_active s2 =>
+  canonical_a_active a =>
+  KeygenM23FinalizeArraySemantics.finalize_reachable_inputs
+    bp s2 a.
+proof.
+move=> hbp hs2 ha.
+rewrite /KeygenM23FinalizeArraySemantics.finalize_reachable_inputs.
+move=> i hi.
+rewrite /KeygenM23FinalizeArraySemantics.reachable_word_inputs.
+split.
++ exact (mode2_output_repr_bound16_word bp mat p0 p1 p2 i hbp hi).
+split.
++ exact (hs2 i hi).
++ exact (ha i hi).
+qed.
+
+op actual_snapshot_mod2q_zero
+    (pre_bp s2 a b1 adjusted : BArray8192.t) : bool =
+  forall i,
+    0 <= i < KeygenM23MatrixSpec.mode2_b_words_i =>
+    Mode2KeygenSnapshotAlgebra.congruent_mod_2q
+      (2 * (W32.to_uint (BArray8192.get32 a i) -
+              2 * W32.to_uint (BArray8192.get32 b1 i)) +
+       2 * W32.to_sint (BArray8192.get32 pre_bp i) +
+       2 * W32.to_sint (BArray8192.get32 adjusted i))
+      0.
+
+op actual_snapshot_low_high_decomposition
+    (pre_bp s2 a b1 adjusted : BArray8192.t) : bool =
+  forall i,
+    0 <= i < KeygenM23MatrixSpec.mode2_b_words_i =>
+    let r = KeygenM23FinalizeArraySemantics.raw_residue
+      (BArray8192.get32 pre_bp i)
+      (BArray8192.get32 s2 i)
+      (BArray8192.get32 a i) in
+    let b0 = KeygenM23FinalizeSemantics.vk_low_int r in
+    r = 2 * W32.to_uint (BArray8192.get32 b1 i) + b0 /\
+    -1 <= b0 <= 1 /\
+    W32.to_sint (BArray8192.get32 adjusted i) =
+      W32.to_sint (BArray8192.get32 s2 i) - b0.
+
+lemma finalize_semantic_output_low_high_decomposition
+    (pre_bp s2 a b1 adjusted : BArray8192.t) :
+  KeygenM23FinalizeArraySemantics.finalize_semantic_output
+    pre_bp s2 a b1 adjusted =>
+  actual_snapshot_low_high_decomposition pre_bp s2 a b1 adjusted.
+proof.
+rewrite /KeygenM23FinalizeArraySemantics.finalize_semantic_output.
+move=> [hwords _].
+rewrite /actual_snapshot_low_high_decomposition => i hi /=.
+have [hb1 hadjusted] := hwords i hi.
+have hrange :
+    0 <= KeygenM23FinalizeArraySemantics.raw_residue
+      (BArray8192.get32 pre_bp i)
+      (BArray8192.get32 s2 i)
+      (BArray8192.get32 a i) < Mode2KeygenSnapshotAlgebra.q.
++ rewrite /KeygenM23FinalizeArraySemantics.raw_residue
+          /Mode2KeygenSnapshotAlgebra.q.
+  apply modz_cmp.
+  by rewrite /KeygenM23FinalizeSemantics.q.
+have hdecompose :=
+  Mode2KeygenSnapshotAlgebra.snapshot_residue_exact_low_high
+    (KeygenM23FinalizeArraySemantics.raw_residue
+      (BArray8192.get32 pre_bp i)
+      (BArray8192.get32 s2 i)
+      (BArray8192.get32 a i)) hrange.
+move: hdecompose => [hdecompose [hlow _]].
+rewrite /Mode2KeygenSnapshotAlgebra.snapshot_high
+        /Mode2KeygenSnapshotAlgebra.snapshot_low in hdecompose.
+rewrite /Mode2KeygenSnapshotAlgebra.snapshot_low in hlow.
+rewrite hb1.
+split; first exact hdecompose.
+split; first exact hlow.
+exact hadjusted.
+qed.
+
+lemma finalize_semantic_output_snapshot_mod2q_zero
+    (pre_bp s2 a b1 adjusted : BArray8192.t) :
+  KeygenM23FinalizeArraySemantics.finalize_semantic_output
+    pre_bp s2 a b1 adjusted =>
+  actual_snapshot_mod2q_zero pre_bp s2 a b1 adjusted.
+proof.
+rewrite /KeygenM23FinalizeArraySemantics.finalize_semantic_output.
+move=> [hwords _].
+rewrite /actual_snapshot_mod2q_zero => i hi.
+have [hb1 hadjusted] := hwords i hi.
+have halgebra :=
+  Mode2KeygenSnapshotAlgebra.snapshot_expression_from_product_congruent_mod_2q
+    (W32.to_sint (BArray8192.get32 pre_bp i))
+    (W32.to_sint (BArray8192.get32 s2 i))
+    (W32.to_uint (BArray8192.get32 a i))
+    0.
+rewrite hb1 hadjusted.
+move: halgebra.
+rewrite /Mode2KeygenSnapshotAlgebra.snapshot_expression_from_product
+        /Mode2KeygenSnapshotAlgebra.residue_high_from_product
+        /Mode2KeygenSnapshotAlgebra.residue_low_from_product
+        /Mode2KeygenSnapshotAlgebra.snapshot_high
+        /Mode2KeygenSnapshotAlgebra.snapshot_low
+        Mode2KeygenSnapshotAlgebra.array_raw_residue_matches_from_product.
+trivial.
+qed.
+
+module ActualM23MatrixFinalizeSnapshot = {
+  proc run
+      (bp : BArray8192.t, s1hatp : BArray8192.t,
+       mat : BArray32768.t, s1 : BArray8192.t,
+       s2 : BArray8192.t, avec : BArray8192.t)
+      : BArray8192.t * BArray8192.t *
+        BArray8192.t * BArray8192.t = {
+    var pre_bp : BArray8192.t;
+
+    (bp, s1hatp) <@ Parent._kp_m23_matrix
+      (bp, s1hatp, mat, s1,
+       W64.of_int KeygenM23MatrixSpec.mode2_rows_i,
+       W64.of_int KeygenM23MatrixSpec.mode2_cols_i);
+    pre_bp <- bp;
+    (bp, s2) <@ Parent._keypair_finalize_m23
+      (bp, s2, avec,
+       W64.of_int KeygenM23MatrixSpec.mode2_b_words_i);
+    return (pre_bp, s1hatp, bp, s2);
+  }
+}.
+
+lemma actual_m23_matrix_finalize_snapshot
+    (bp0 s1hat0 s10 s20 avec0 : BArray8192.t)
+    (mat0 : BArray32768.t)
+    (p0 p1 p2 : Rq.poly) :
+  hoare [ActualM23MatrixFinalizeSnapshot.run :
+    bp = bp0 /\ s1hatp = s1hat0 /\
+    mat = mat0 /\ s1 = s10 /\ s2 = s20 /\ avec = avec0 /\
+    KeygenM23ArithmeticSpec.matrix_active_bound16 mat0 /\
+    KeygenM23ArithmeticSpec.mode2_input_repr_bound16
+      s10 p0 p1 p2 /\
+    centered_s2_active s20 /\
+    canonical_a_active avec0
+    ==>
+    KeygenM23ArithmeticSpec.mode2_output_repr_bound16
+      res.`1 mat0 p0 p1 p2 /\
+    KeygenM23ArithmeticSpec.mode2_ntt_repr_bound24
+      res.`2 p0 p1 p2 /\
+    KeygenM23FinalizeSpec.finalize_output
+      res.`1 s20 avec0 res.`3 res.`4 /\
+    KeygenM23MatrixSpec.word_tail_frame
+      bp0 res.`1 KeygenM23MatrixSpec.mode2_b_words_i /\
+    KeygenM23MatrixSpec.word_tail_frame
+      s1hat0 res.`2 KeygenM23MatrixSpec.mode2_s1_words_i /\
+    KeygenM23MatrixSpec.word_tail_frame
+      s20 res.`4 KeygenM23MatrixSpec.mode2_b_words_i].
+proof.
+proc.
+seq 1 :
+  (s2 = s20 /\ avec = avec0 /\
+   KeygenM23ArithmeticSpec.mode2_output_repr_bound16
+     bp mat0 p0 p1 p2 /\
+   KeygenM23ArithmeticSpec.mode2_ntt_repr_bound24
+     s1hatp p0 p1 p2 /\
+   KeygenM23MatrixSpec.word_tail_frame
+     bp0 bp KeygenM23MatrixSpec.mode2_b_words_i /\
+   KeygenM23MatrixSpec.word_tail_frame
+     s1hat0 s1hatp KeygenM23MatrixSpec.mode2_s1_words_i /\
+   centered_s2_active s20 /\
+   canonical_a_active avec0).
++ call
+    (TargetKeygenM23Arithmetic.kp_m23_matrix_mode2_arithmetic_correct
+      bp0 s1hat0 mat0 s10 p0 p1 p2).
+  auto => />.
+exlim bp => pre_bp0.
+call
+  (TargetKeygenM23Finalize.keypair_finalize_m23_mode2_correct
+    pre_bp0 s20 avec0).
+auto => />.
+qed.
+
+lemma actual_m23_matrix_finalize_semantic_snapshot
+    (bp0 s1hat0 s10 s20 avec0 : BArray8192.t)
+    (mat0 : BArray32768.t)
+    (p0 p1 p2 : Rq.poly) :
+  hoare [ActualM23MatrixFinalizeSnapshot.run :
+    bp = bp0 /\ s1hatp = s1hat0 /\
+    mat = mat0 /\ s1 = s10 /\ s2 = s20 /\ avec = avec0 /\
+    KeygenM23ArithmeticSpec.matrix_active_bound16 mat0 /\
+    KeygenM23ArithmeticSpec.mode2_input_repr_bound16
+      s10 p0 p1 p2 /\
+    centered_s2_active s20 /\
+    canonical_a_active avec0
+    ==>
+    KeygenM23ArithmeticSpec.mode2_output_repr_bound16
+      res.`1 mat0 p0 p1 p2 /\
+    KeygenM23ArithmeticSpec.mode2_ntt_repr_bound24
+      res.`2 p0 p1 p2 /\
+    KeygenM23FinalizeSpec.finalize_output
+      res.`1 s20 avec0 res.`3 res.`4 /\
+    KeygenM23FinalizeArraySemantics.finalize_semantic_output
+      res.`1 s20 avec0 res.`3 res.`4 /\
+    actual_snapshot_low_high_decomposition
+      res.`1 s20 avec0 res.`3 res.`4 /\
+    KeygenM23FinalizeHAETAEBridge.finalize_haetae_semantic_output
+      res.`1 s20 avec0 res.`3 res.`4 /\
+    actual_snapshot_mod2q_zero
+      res.`1 s20 avec0 res.`3 res.`4 /\
+    KeygenM23MatrixSpec.word_tail_frame
+      bp0 res.`1 KeygenM23MatrixSpec.mode2_b_words_i /\
+    KeygenM23MatrixSpec.word_tail_frame
+      bp0 res.`3 KeygenM23MatrixSpec.mode2_b_words_i /\
+    KeygenM23MatrixSpec.word_tail_frame
+      s1hat0 res.`2 KeygenM23MatrixSpec.mode2_s1_words_i /\
+    KeygenM23MatrixSpec.word_tail_frame
+      s20 res.`4 KeygenM23MatrixSpec.mode2_b_words_i].
+proof.
+conseq
+  (actual_m23_matrix_finalize_snapshot
+    bp0 s1hat0 s10 s20 avec0 mat0 p0 p1 p2) => //=.
+move=> &m hpre result hpost.
+move: hpre =>
+  [_ [_ [_ [_ [_ [_ [_ [_ [hcenter hcanonical]]]]]]]]].
+move: hpost =>
+  [hout [hntt [hfinal [hpreframe [hhatframe hs2frame]]]]].
+have hreachable :=
+  finalize_reachable_inputs_from_matrix_output
+    result.`1 s20 avec0 mat0 p0 p1 p2
+    hout hcenter hcanonical.
+have hsemantic :=
+  KeygenM23FinalizeArraySemantics.finalize_output_semantics
+    result.`1 s20 avec0 result.`3 result.`4
+    hreachable hfinal.
+have hhaetae :=
+  KeygenM23FinalizeHAETAEBridge.finalize_semantic_output_haetae
+    result.`1 s20 avec0 result.`3 result.`4 hsemantic.
+have hdecomposition :=
+  finalize_semantic_output_low_high_decomposition
+    result.`1 s20 avec0 result.`3 result.`4 hsemantic.
+have hmod2q :=
+  finalize_semantic_output_snapshot_mod2q_zero
+    result.`1 s20 avec0 result.`3 result.`4 hsemantic.
+have hfinalframe :
+    KeygenM23MatrixSpec.word_tail_frame
+      result.`1 result.`3 KeygenM23MatrixSpec.mode2_b_words_i.
++ move: hsemantic.
+  rewrite /KeygenM23FinalizeArraySemantics.finalize_semantic_output.
+  by move=> [_ [h _]].
+have hcomposedframe :=
+  KeygenM23MatrixSpec.word_tail_frame_trans
+    bp0 result.`1 result.`3 KeygenM23MatrixSpec.mode2_b_words_i
+    hpreframe hfinalframe.
+split; first exact hout.
+split; first exact hntt.
+split; first exact hfinal.
+split; first exact hsemantic.
+split; first exact hdecomposition.
+split; first exact hhaetae.
+split; first exact hmod2q.
+split; first exact hpreframe.
+split; first exact hcomposedframe.
+split; first exact hhatframe.
+exact hs2frame.
+qed.
+
+end Mode2KeygenCoreEquation.
